add macros

examples/wrapping_add.c
@@ -1,0 +1,17 @@
+#include <stddef.h>
+#include <refinedc.h>
+
+#define WRAPPING_ADD(it1, it2, a, b) RC_MACRO(WrappingAdd, (a) + (b), \
+     RC_MACRO_ARG(it1), RC_MACRO_ARG(it2), RC_MACRO_EXPR(a), RC_MACRO_EXPR(b))
+
+//@rc::import wrapping_def from refinedc.examples.wrapping_add (for code only)
+//@rc::import wrapping_rules from refinedc.examples.wrapping_add
+
+[[rc::parameters("a : Z", "b : Z", "c : Z")]]
+[[rc::args("a @ int<size_t>", "b @ int<size_t>", "c @ int<size_t>")]]
+[[rc::requires("{(b + c < int_modulus size_t)}")]]
+/* We don't want to add the following: [[rc::requires("{(a + b < int_modulus size_t)}")]] */
+[[rc::returns("{((a + (b + c)) `mod` int_modulus size_t)} @ int<size_t>")]]
+size_t wrapping_add(size_t a, size_t b, size_t c) {
+  return WRAPPING_ADD(size_t, size_t, a, (b + c));
+}
