frontend/coq_ast.ml
@@ -52,6 +52,7 @@ and expr_aux =
   | GetMember of expr * string * bool (* From_union? *) * string
   | AnnotExpr of int * coq_expr * expr
   | Struct    of string * (string * expr) list
+  | Macro     of string * string list * expr list * expr
 
 type stmt = stmt_aux Location.located
 and stmt_aux =
