examples/proofs/wrapping_add/generated_proof_wrapping_add.v
@@ -1,0 +1,26 @@
+From refinedc.typing Require Import typing.
+From refinedc.examples.wrapping_add Require Import generated_code.
+From refinedc.examples.wrapping_add Require Import generated_spec.
+From refinedc.examples.wrapping_add Require Import wrapping_rules.
+Set Default Proof Using "Type".
+
+(* Generated from [examples/wrapping_add.c]. *)
+Section proof_wrapping_add.
+  Context `{!typeG Σ} `{!globalG Σ}.
+
+  (* Typing proof for [wrapping_add]. *)
+  Lemma type_wrapping_add :
+    ⊢ typed_function impl_wrapping_add type_of_wrapping_add.
+  Proof.
+    start_function "wrapping_add" ([[a b] c]) => arg_a arg_b arg_c.
+    split_blocks ((
+      ∅
+    )%I : gmap label (iProp Σ)) ((
+      ∅
+    )%I : gmap label (iProp Σ)).
+    - repeat liRStep; liShow.
+      all: print_typesystem_goal "wrapping_add" "#0".
+    Unshelve. all: sidecond_hook; prepare_sideconditions; normalize_and_simpl_goal; try solve_goal; unsolved_sidecond_hook.
+    all: print_sidecondition_goal "wrapping_add".
+  Qed.
+End proof_wrapping_add.
