examples/proofs/wrapping_add/generated_spec.v
@@ -1,0 +1,16 @@
+From refinedc.typing Require Import typing.
+From refinedc.examples.wrapping_add Require Import generated_code.
+From refinedc.examples.wrapping_add Require Import wrapping_rules.
+Set Default Proof Using "Type".
+
+(* Generated from [examples/wrapping_add.c]. *)
+Section spec.
+  Context `{!typeG Σ} `{!globalG Σ}.
+
+  (* Type definitions. *)
+
+  (* Specifications for function [wrapping_add]. *)
+  Definition type_of_wrapping_add :=
+    fn(∀ (a, b, c) : Z * Z * Z; (a @ (int (size_t))), (b @ (int (size_t))), (c @ (int (size_t))); ⌜(b + c < int_modulus size_t)⌝)
+      → ∃ () : (), ((((a + (b + c)) `mod` int_modulus size_t)) @ (int (size_t))); True.
+End spec.
