examples/proofs/wrapping_add/wrapping_def.v
@@ -1,0 +1,13 @@
+From refinedc.lang Require Import notation tactics.
+Set Default Proof Using "Type".
+
+Definition WrappingAdd (it1 it2 : int_type) (es : list expr) : expr :=
+  match es with
+  | [e1 ; e2] => e1 +{IntOp it1, IntOp it2} e2
+  | _ => Val VOID
+  end%E.
+
+Program Instance WrappingAdd_wf it1 it2 : MacroWfSubst (WrappingAdd it1 it2).
+Next Obligation. move => ???? [|?[|?[|??]]]//. Qed.
+
+Typeclasses Opaque WrappingAdd.
