examples/proofs/wrapping_add/wrapping_rules.v
@@ -1,0 +1,39 @@
+From refinedc.typing Require Import typing.
+From refinedc.examples.wrapping_add Require Export wrapping_def.
+Set Default Proof Using "Type".
+
+Section type.
+  Context `{!typeG Σ}.
+
+  Lemma macro_wrapping_add it1 it2 e1 e2 T:
+    typed_val_expr e1 (λ v1 ty1, typed_val_expr e2 (λ v2 ty2,
+      ∃ n1 n2, subsume (v1 ◁ᵥ ty1) (v1 ◁ᵥ n1 @ int it1) (
+               subsume (v2 ◁ᵥ ty2) (v2 ◁ᵥ n2 @ int it2) (
+               (⌜n1 ∈ it1⌝ -∗ ⌜n2 ∈ it2⌝ -∗ ⌜it1 = it2⌝ ∗ ⌜it_signed it1 = false⌝ ∗ (
+               ∀ v, T v (t2mt (((n1 + n2) `mod` int_modulus it1) @ int it1)))))))) -∗
+    typed_macro_expr (WrappingAdd it1 it2) [e1 ; e2] T.
+  Proof.
+    iIntros "HT". rewrite /typed_macro_expr/WrappingAdd. iApply type_bin_op.
+    iIntros (Φ) "HΦ". iApply "HT". iIntros (v1 ty1) "Hty1 HT". iApply ("HΦ" with "Hty1"). clear.
+    iIntros (Φ) "HΦ". iApply "HT". iIntros (v2 ty2) "Hty2 HT". iApply ("HΦ" with "Hty2"). clear.
+    iIntros "Hty1 Hty2". iDestruct "HT" as (n1 n2) "HT".
+    iDestruct ("HT" with "Hty1") as (Hv1) "HT".
+    iDestruct ("HT" with "Hty2") as (Hv2) "HT".
+    iIntros (Φ) "HΦ".
+    iDestruct ("HT" with "[] []" ) as (??) "HT".
+    1-2: iPureIntro; by apply: val_of_int_in_range.
+    have /val_of_int_is_some[v Hv] : ((n1 + n2) `mod` int_modulus it1) ∈ it1 by apply int_modulus_mod_in_range.
+    move: Hv1 Hv2 => /val_to_of_int Hv1 /val_to_of_int Hv2. subst it2.
+    iApply (wp_binop_det v). iSplit.
+    - iIntros (σ v') "_ !%". split.
+      + inversion 1; simplify_eq/=.
+        by destruct it1 as [? []]; simplify_eq/=.
+      + move => ->. econstructor => //.
+        by destruct it1 as [? []]; simplify_eq/=.
+    - iIntros "!>". iApply "HΦ"; last done. by iPureIntro.
+  Qed.
+
+  Global Instance macro_wrapping_add_inst it1 it2 e1 e2 :
+    TypedMacroExpr (WrappingAdd it1 it2) [e1 ; e2] :=
+    λ T, i2p (macro_wrapping_add it1 it2 e1 e2 T).
+End type.
